fewer hand edits

src/tls13formats/handshake_data.rs
@@ -1,6 +1,8 @@
 #[cfg(feature = "hax-pv")]
 use hax_lib::{pv_constructor, pv_handwritten};
 
+use hax_lib::ToInt;
+
 use crate::tls13utils::{
     check_eq1, encode_length_u24, eq1, length_u24_encoded, parse_failed, tlserr, Bytes, TLSError,
     U8,
@@ -99,8 +101,11 @@ impl HandshakeData {
     /// parsing is unsuccessful or the type of the parsed message disagrees with the
     /// expected type.
     #[hax_lib::ensures(|result| match result {
-        Result::Ok(d) => self.len() >= 4 && d.len() == self.len() - 4,
-        _ => true })]
+                                    Result::Ok(d) => {
+                                        let self_: Self = {hax_lib::fstar::unsafe_expr!("self")};
+                                        self_.len() >= 4 && 
+                                        self_.len() - 4 == d.len()},
+                                    _ => true })]
     pub(crate) fn as_handshake_message(
         &self,
         expected_type: HandshakeType,
@@ -123,9 +128,15 @@ impl HandshakeData {
     /// payload. Returns a [TLSError] if the payload is too short to contain a
     /// handshake message or if the payload is shorter than the expected length
     /// encoded in its first three bytes.
+    ///
+    /// We needed to uglify the ensures here because of: https://github.com/cryspen/hax/issues/1276
     #[hax_lib::ensures(|result| match result {
-                                        Result::Ok((m,r)) => m.len() >= 4 && self.len() >= m.len() && self.len() - m.len() == r.len(),
-                                        _ => true })]
+                                    Result::Ok((m,r)) => {
+                                        let self_: Self = {hax_lib::fstar::unsafe_expr!("self")};
+                                        m.len() >= 4 &&
+                                        self_.len() >= m.len() && 
+                                        self_.len() - m.len() == r.len()},
+                                    _ => true })]
     pub(crate) fn next_handshake_message(&self) -> Result<(Self, Self), TLSError> {
         if (self.len()) < 4 {
             tlserr(parse_failed())
@@ -177,11 +188,10 @@ impl HandshakeData {
     /// Beginning at offset `start`, attempt to find a message of type `handshake_type` in `payload`.
     ///
     /// Returns `true`` if `payload` contains a message of the given type, `false` otherwise.
-    ///
-    /// For termination proof in F*: we need to hand-edit and add:
-    /// (decreases (Seq.length self._0._0 - v start))
-    /// https://github.com/cryspen/hax/issues/1233
-    #[hax_lib::requires(fstar!(r#"Seq.length self._0._0 >= v start"#))]
+    #[hax_lib::requires({let self_: Self = {hax_lib::fstar::unsafe_expr!("self")};
+                         self_.len() >= start})]
+    #[hax_lib::decreases({let self_: Self = {hax_lib::fstar::unsafe_expr!("self")};
+                          self_.len().to_int() - start.to_int()})]
     pub(crate) fn find_handshake_message(
         &self,
         handshake_type: HandshakeType,
